\documentclass{article}
\usepackage{amsfonts}
\usepackage{amsmath}
\usepackage{amssymb}
\usepackage{hyperref}
\usepackage{mathrsfs}
\parindent=0pt

\def\upint{\mathchoice%
    {\mkern13mu\overline{\vphantom{\intop}\mkern7mu}\mkern-20mu}%
    {\mkern7mu\overline{\vphantom{\intop}\mkern7mu}\mkern-14mu}%
    {\mkern7mu\overline{\vphantom{\intop}\mkern7mu}\mkern-14mu}%
    {\mkern7mu\overline{\vphantom{\intop}\mkern7mu}\mkern-14mu}%
  \int}
\def\lowint{\mkern3mu\underline{\vphantom{\intop}\mkern7mu}\mkern-10mu\int}

\begin{document}

\textbf{\Large Chapter 15: Bernoulli Numbers} \\\\



\emph{Author: Meng-Gen Tsai} \\
\emph{Email: plover@gmail.com} \\\\



% https://dms.umontreal.ca/~mlalin/bernoulli.pdf
% http://cds.iisc.ac.in/faculty/amohanty/SE288/bn.pdf



\textbf{Supplement.} Equation (4) on page 231.
\emph{Prove that $$x \cot x = 1 - 2 \sum_{n=1}^{\infty} \frac{x^2}{n^2 \pi^2 - x^2}.$$} \\

\emph{Proof (Exercise 6.73 in the book Graham, Knuth and Patashnik,
Concrete Mathematics, Second Edition).}

\begin{enumerate}
\item[(1)]
\emph{Show that $$\cot x
= \frac{1}{2^n} \sum_{k=0}^{2^{n} - 1} \cot \frac{x + k\pi}{2^n}$$
for all integers $n \geq 1$.}
Notice that
\begin{align*}
\cot(x + \pi) &= \cot x, \\
\cot\left( x + \frac{\pi}{2} \right) &= -\tan x, \\
\cot x &= \frac{1}{2} \left( \cot\frac{x}{2} - \tan\frac{x}{2} \right).
\end{align*}
Use mathematical induction.
The case $n = 1$ is the same as the note.
Assume the case $n = m$ holds.
For $n = m+1$,
\begin{align*}
\sum_{k=0}^{2^{m+1} - 1} \cot \frac{x + k\pi}{2^{m+1}}
&= \sum_{k=0}^{2^{m} - 1} \cot \frac{x + k\pi}{2^{m+1}}
+ \sum_{k=2^{m}}^{2^{m+1} - 1} \cot \frac{x + k\pi}{2^{m+1}} \\
&= \sum_{k=0}^{2^{m} - 1} \cot \frac{x + k\pi}{2^{m+1}}
+ \sum_{k=0}^{2^{m} - 1} \cot \frac{x + (2^{m} + k)\pi}{2^{m+1}} \\
&= \sum_{k=0}^{2^{m} - 1} \cot \frac{x + k\pi}{2^{m+1}}
+ \sum_{k=0}^{2^{m} - 1} \cot \left( \frac{x + k\pi}{2^{m+1}} + \frac{\pi}{2} \right) \\
&= \sum_{k=0}^{2^{m} - 1}
\left( \cot \frac{x + k\pi}{2^{m+1}} - \tan \frac{x + k\pi}{2^{m+1}} \right) \\
&= \sum_{k=0}^{2^{m} - 1}
\left( \cot \frac{x + k\pi}{2^{m+1}} - \tan \frac{x + k\pi}{2^{m+1}} \right) \\
&= 2 \sum_{k=0}^{2^{m} - 1} \cot \frac{x + k\pi}{2^{m}}.
\end{align*}
Therefore,
\begin{align*}
\frac{1}{2^{m+1}} \sum_{k=0}^{2^{m+1} - 1} \cot \frac{x + k\pi}{2^{m+1}}
&= \frac{1}{2^{m+1}} \cdot 2 \sum_{k=0}^{2^{m} - 1} \cot \frac{x + k\pi}{2^{m}} \\
&= \frac{1}{2^{m}} \sum_{k=0}^{2^{m} - 1} \cot \frac{x + k\pi}{2^{m}} \\
&= \cot x.
\end{align*}
\item[(2)]
By rearranging the index of summation of the identity in (1), we have
$$x \cot x
= \frac{x}{2^n} \cot \frac{x}{2^n} - \frac{x}{2^n} \tan \frac{x}{2^n}
+ \sum_{k=1}^{2^{n-1} - 1} \frac{x}{2^n}
\left( \cot \frac{x + k\pi}{2^n} + \cot \frac{x - k\pi}{2^n} \right)$$
for all integers $n \geq 1$.
\item[(3)]
Notice that $\lim_{x \rightarrow 0} x \cot x = 1$.
Let $n \rightarrow \infty$, the result is established.
\end{enumerate}
$\Box$ \\\\



\textbf{Exercise 15.1.}
\emph{Using the definition of the Bernoulli number show
$B_{10} = \frac{5}{66}$ and $B_{12} = -\frac{691}{2730}$.} \\

\emph{Proof.}
\begin{enumerate}
\item[(1)]
It is known that
$B_1 = -\frac{1}{2}$,
$B_2 = \frac{1}{6}$,
$B_4 = -\frac{1}{30}$,
$B_6 = \frac{1}{42}$,
and $B_m = 0$ for odd $m > 1$.
\item[(2)]
Recall the implicit recurrence relation,
$$\sum_{k = 0}^{m} {m+1 \choose k} B_k = [m = 0],$$
where $[m = 0]$ is the Iverson brackets which is equal to
the Kronecker delta $\delta_{m0}$.
\item[(3)]
So
\begin{align*}
0 &= 1 + 9 B_1 + 36 B_2 + 84 B_3 + 126 B_4 + 126 B_5 + 84 B_6 + 36 B_7 + 9 B_8, \\
0 &= 1 + 9 B_1 + 36 B_2 + 126 B_4 + 84 B_6 + 9 B_8, \\
0 &= 1 + 9 \left( -\frac{1}{2} \right)
+ 36 \left( \frac{1}{6} \right)
+ 126 \left( -\frac{1}{30} \right)
+ 84 \left( \frac{1}{42} \right)
+ 9 B_8, \\
0 &= \frac{3}{10} + 9B_8,
\end{align*}
Thus $B_8 = -\frac{1}{30}$. \\
\item[(4)]
Again,
\begin{align*}
0 =& 1 + 11 B_1 + 55 B_2 + 165 B_3 + 330 B_4 + 462 B_5 + 462 B_6 + \\
   & 330 B_7 + 165 B_8 + 55 B_9 + 11 B_{10}, \\
0 =& 1 + 11 B_1 + 55 B_2 + 330 B_4 + 462 B_6 + 165 B_8 + 11 B_{10}, \\
0 =& 1 + 11 \left( -\frac{1}{2} \right) +
     55 \left( \frac{1}{6} \right) +
     330 \left( -\frac{1}{30} \right) +
     462 \left( \frac{1}{42} \right) + \\
   & 165 \left( -\frac{1}{30} \right) +
     11 B_{10}, \\
0 =& -\frac{5}{6} + 11 B_{10},
\end{align*}
Thus $B_{10} = \frac{5}{66}$. \\
\item[(4)]
Finally,
\begin{align*}
0 =& 1 + 13 B_1 + 78 B_2 + 286 B_3 + 715 B_4 + 1287 B_5 + 1716 B_6 + \\
   & 1716 B_7 + 1287 B_8 + 715 B_9 + 286 B_{10} + 78 B_{11} + 13 B_{12}, \\
0 =& 1 + 13 B_1 + 78 B_2 + 715 B_4 + 1716 B_6 + 1287 B_8 + 286 B_{10} + 13 B_{12}, \\
0 =& 1 + 13 \left( -\frac{1}{2} \right) +
     78 \left( \frac{1}{6} \right) +
     715 \left( -\frac{1}{30} \right) +
     1716 \left( \frac{1}{42} \right) + \\
   & 1287 \left( -\frac{1}{30} \right) +
     286 \left( \frac{5}{66} \right) +
     13 B_{12}, \\
0 =& \frac{691}{210} + 13 B_{12},
\end{align*}
Thus $B_{12} = -\frac{691}{2730}$.
\end{enumerate}
$\Box$\\\\



\textbf{Exercise 15.2.}
\emph{If $a \in \mathbb{Z}$,
show $a(a^m - 1)B_m \in \mathbb{Z}$ for all $m > 0$.} \\

\emph{Proof.}
\begin{enumerate}
\item[(1)] \emph{Trivial cases.}
If $m = 1$, $a(a - 1) B_1 = -\frac{1}{2} a(a - 1) \in \mathbb{Z}$ for any $a \in \mathbb{Z}$.
For odd $m > 1$, $B_m = 0$ or $a(a^m - 1)B_m = 0 \in \mathbb{Z}$ (Proposition 15.1.1). \\
\item[(2)] \emph{Consider that $m > 1$ and even.}
By Theorem 3,
$$B_{2m} + \sum_{p-1 \mid 2m} \frac{1}{p} \in \mathbb{Z}$$
where the sum is over all primes $p$ such that $p-1 \mid 2m$.
So it suffices to show
$$a(a^{2m} - 1) \sum_{p-1 \mid 2m} \frac{1}{p} \in \mathbb{Z}, $$
or
$$a(a^{2m} - 1) \frac{1}{p} \in \mathbb{Z}$$
for any $a \in \mathbb{Z}$ and any prime $p$ such that $p-1 \mid 2m$.
\item[(3)] \emph{Consider all possible $a$.}
If $p \mid a$, it is trivial.
If $p \nmid a$, $a^{p - 1} \equiv 1 \: (p)$ by Fermat's Little Theorem,
or $a^{2m} \equiv 1 \: (p)$ by $p-1 \mid 2m$.
In any cases, $a(a^{2m} - 1)\frac{1}{p} \in \mathbb{Z}$.
\end{enumerate}
$\Box$ \\\\



\textbf{Exercise 15.6.}
\emph{For $m \geq 3$, show $|B_{2m+2}| > |B_{2m}|$. (Hint: Use Theorem 2.)} \\

\emph{Proof.}
By Theorem 2,
$$2 \zeta(2m) = (-1)^{m+1} \frac{(2\pi)^{2m}}{(2m)!} B_{2m}.$$
Thus,
$$\frac{|B_{2m+2}|}{|B_{2m}|}
= \frac{\zeta(2m+2)(2m+2)(2m+1)}{\zeta(2m)(2\pi)^2}
> \frac{1 \cdot 8 \cdot 7}{\zeta(6) \cdot (2\pi)^2}
= \frac{13230}{\pi^8}
> 1,$$
or $|B_{2m+2}| > |B_{2m}|$.
$\Box$ \\\\



\textbf{Exercise 15.8.}
\emph{Consider the power series expansion of $\tan x$ about the origin;
$$\sum_{k=1}^{\infty} T_k \frac{x^{2k - 1}}{(2k - 1)!}.$$
Show $$T_k = (-1)^{k-1} \frac{B_{2k}}{2k} (2^{2k} - 1) 2^{2k}.$$
Note that $T_k \in \mathbb{Z}$ for all $k$ by Exercise 3.} \\

\emph{Proof.}
\begin{enumerate}
\item[(1)]
By the equation (6) on page 232,
$$x \cot x = 1 + \sum_{k=2}^{\infty} B_k \frac{(2ix)^k}{k!}.$$
Since $B_k = 0$ for odd $k > 1$,
$$x \cot x
= 1 + \sum_{k=1}^{\infty} B_{2k} \frac{(2ix)^{2k}}{(2k)!}
= 1 + \sum_{k=1}^{\infty} \frac{(-1)^k 2^{2k}B_{2k}}{(2k)!} x^{2k},$$
or
$$\cot x
= \frac{1}{x} + \sum_{k=1}^{\infty} \frac{(-1)^k 2^{2k}B_{2k}}{(2k)!} x^{2k-1}.$$
Combine the first term $\frac{1}{x}$ into the summation,
$$\cot x = \sum_{k=0}^{\infty} \frac{(-1)^k 2^{2k}B_{2k}}{(2k)!} x^{2k-1}.$$
\item[(2)]
Note that $\tan x = \cot x - 2 \cot(2x)$.
By (1),
\begin{align*}
\tan x
&= \sum_{k=0}^{\infty} \frac{(-1)^k 2^{2k}B_{2k}}{(2k)!} x^{2k-1}
- 2 \sum_{k=0}^{\infty} \frac{(-1)^k 2^{2k}B_{2k}}{(2k)!} (2x)^{2k-1} \\
&= \sum_{k=0}^{\infty} \frac{(-1)^k (1 - 2^{2k}) 2^{2k} B_{2k}}{(2k)!} x^{2k-1} \\
&= \sum_{k=1}^{\infty} \frac{(-1)^k (1 - 2^{2k}) 2^{2k} B_{2k}}{(2k)!} x^{2k-1}.
\end{align*}
Write $T_k = (-1)^{k-1} (2^{2k} - 1) 2^{2k} \frac{B_{2k}}{2k}$.
Therefore, $\tan x = \sum_{k=1}^{\infty} T_k \frac{x^{2k - 1}}{(2k - 1)!}$.
\end{enumerate}
By Exercise 3, $(2^{2k} - 1) 2^{2k} \frac{B_{2k}}{2k} \in \mathbb{Z}$,
or $T_k \in \mathbb{Z}$ for all $k$.
$\Box$ \\\\



\textbf{Exercise 15.13.}
\emph{Show $B_m(x+1) - B_m(x) = mx^{m-1}$.} \\

\emph{Proof.}
Let $f(t, x) = \frac{te^{tx}}{e^t - 1}$.
\begin{enumerate}
\item[(1)]
$$f(t, x+1) - f(t, x)
= \frac{te^{t(x+1)}}{e^t - 1} - \frac{te^{tx}}{e^t - 1}
= te^{tx}.$$
Expand $te^{tx}$ in a power series about the origin as follows
\begin{align*}
te^{tx}
&= t \sum_{m=0}^{\infty} x^m \frac{t^m}{m!} \\
&= \sum_{m=0}^{\infty} x^m \frac{t^{m+1}}{m!} \\
&= \sum_{m=1}^{\infty} x^{m-1} \frac{t^m}{(m-1)!} \\
&= \sum_{m=1}^{\infty} mx^{m-1} \frac{t^m}{m!} \\
&= \sum_{m=0}^{\infty} mx^{m-1} \frac{t^m}{m!}.
\end{align*}
So,
$$f(t, x+1) - f(t, x) = \sum_{m=0}^{\infty} mx^{m-1} \frac{t^m}{m!}.$$
\item[(2)]
By Exercise 15.12,
\begin{align*}
f(t, x+1) - f(t, x)
&= \sum_{m=0}^{\infty} B_m(x+1) \frac{t^m}{m!}
- \sum_{m=0}^{\infty} B_m(x) \frac{t^m}{m!} \\
&= \sum_{m=0}^{\infty} (B_m(x+1) - B_m(x)) \frac{t^m}{m!}.
\end{align*}
\end{enumerate}
By (1)(2), comparing coefficients of $t^m$ yields
$$mx^{m-1} = B_m(x+1) - B_m(x).$$
$\Box$ \\\\



\textbf{Exercise 15.14.}
\emph{Use Exercise 13 to give a new proof of Theorem 1:
$$S_m(n) = \frac{1}{m+1}(B_{m+1}(n) - B_{m+1}).$$}

\emph{Proof.}
By Exercise 13,
$$B_{m+1}(k) - B_{m+1}(k-1) = (m+1)(k-1)^m$$
for any $k$.
So,
\begin{align*}
\sum_{k=1}^{n} (B_{m+1}(k) - B_{m+1}(k-1))
&= \sum_{k=1}^{n} (m+1)(k-1)^m, \\
B_{m+1}(n) - B_{m+1}(0)
&= (m+1)S_m(n).
\end{align*}
Note that $B_{m+1}(0) = B_{m+1}$ for any $m$.
So Theorem 1 is established by a new proof.
$\Box$ \\\\



\textbf{Exercise 15.16.}
\emph{For $n \geq 1$, show $\frac{d}{dx}B_n(x) = nB_{n-1}(x)$.} \\

\emph{Proof.}
For $n \geq 1$,
$$\frac{d}{dx}B_n(x)
= \sum_{k=0}^{n}(n - k) {n \choose k} B_k x^{n - k - 1}
= \sum_{k=0}^{n-1}(n - k) {n \choose k} B_k x^{n - k - 1}.$$
Note that
$$(n-k) {n \choose k} = n {n-1 \choose k}.$$
So
\begin{align*}
\frac{d}{dx}B_n(x)
&= \sum_{k=0}^{n-1} n {n-1 \choose k} B_k x^{n - k - 1} \\
&= n \sum_{k=0}^{n-1} {n-1 \choose k} B_k x^{n - k - 1} \\
&= n B_{n-1}(x).
\end{align*}

$\Box$ \\\\



\end{document}