\documentclass{article}
\usepackage{amsfonts}
\usepackage{amsmath}
\usepackage{amssymb}
\usepackage{hyperref}
\usepackage{mathrsfs}
\parindent=0pt

\def\upint{\mathchoice%
    {\mkern13mu\overline{\vphantom{\intop}\mkern7mu}\mkern-20mu}%
    {\mkern7mu\overline{\vphantom{\intop}\mkern7mu}\mkern-14mu}%
    {\mkern7mu\overline{\vphantom{\intop}\mkern7mu}\mkern-14mu}%
    {\mkern7mu\overline{\vphantom{\intop}\mkern7mu}\mkern-14mu}%
  \int}
\def\lowint{\mkern3mu\underline{\vphantom{\intop}\mkern7mu}\mkern-10mu\int}

\begin{document}

\textbf{\Large Chapter 3: Operators} \\\\



\emph{Author: Meng-Gen Tsai} \\
\emph{Email: plover@gmail.com} \\\\



%%%%%%%%%%%%%%%%%%%%%%%%%%%%%%%%%%%%%%%%%%%%%%%%%%%%%%%%%%%%%%%%%%%%%%%%%%%%%%%%



\textbf{Problem 3.6.}
\emph{Prove that $\hat{A} + \hat{B} = \hat{B} + \hat{A}$. } \\

Two operators $\hat{A}$ and $\hat{B}$ are said to be equal if
$\hat{A}f = \hat{B}f$ for all functions $f$. \\

\emph{Proof.}
$$(\hat{A} + \hat{B})f = \hat{A}f + \hat{B}f
= \hat{B}f + \hat{A}f = (\hat{B} + \hat{A})f$$
holds for any function $f$.
By definition,
$\hat{A} + \hat{B} = \hat{B} + \hat{A}$.
$\Box$ \\\\



%%%%%%%%%%%%%%%%%%%%%%%%%%%%%%%%%%%%%%%%%%%%%%%%%%%%%%%%%%%%%%%%%%%%%%%%%%%%%%%%



\textbf{Problem 3.7.}
\emph{Let $\hat{D} = d/dx$.
Verify that $(\hat{D}+x)(\hat{D}-x) = \hat{D}^2-x^2-1$. } \\

\emph{Proof.}
\begin{align*}
((\hat{D}+x)(\hat{D}-x))f
&= (\hat{D}+x)((\hat{D}-x)f) \\
&= (\hat{D}+x)(f'-xf) \\
&= (f'-xf)' + x(f'-xf) \\
&= (f''-f-xf') + (xf'-x^2f) \\
&= f''-f-x^2f \\
&= (\hat{D}^2-x^2-1)f
\end{align*}
holds for any function $f$.
By definition,
$(\hat{D}+x)(\hat{D}-x) = \hat{D}^2-x^2-1$.
$\Box$ \\\\



%%%%%%%%%%%%%%%%%%%%%%%%%%%%%%%%%%%%%%%%%%%%%%%%%%%%%%%%%%%%%%%%%%%%%%%%%%%%%%%%



\textbf{Problem 3.27.}
\emph{Evaluate the commutators}
\begin{enumerate}
\item[(a)]
$[\hat{x}, \hat{p}_x]$;
\item[(b)]
$[\hat{x}, \hat{p}_x^2]$;
\item[(c)]
$[\hat{x}, \hat{p}_y]$;
\item[(d)]
$[\hat{x}, \hat{V}(x,y,z)]$;
\item[(e)]
\emph{$[\hat{x}, \hat{H}]$, where the Hamiltonian operator is
$$\hat{H} = -\frac{\hbar}{2m}\left(
\frac{\partial^2}{\partial x^2} + \frac{\partial^2}{\partial y^2} + \frac{\partial^2}{\partial z^2}
\right) + V(x,y,z);$$}
\item[(f)]
$[\hat{x}\hat{y}\hat{z}, \hat{p}_x^2]$. \\
\end{enumerate}

\emph{Proof of (a).}
\begin{align*}
[\hat{x}, \hat{p}_x]f
&= (\hat{x}\hat{p}_x - \hat{p}_x \hat{x})f \\
&= (\hat{x}\hat{p}_x)f - (\hat{p}_x \hat{x})f \\
&= (\hat{x})\left( \frac{\hbar}{i}\frac{\partial f}{\partial x} \right)
  - (\hat{p}_x)(xf) \\
&= x \frac{\hbar}{i}\frac{\partial f}{\partial x}
  - \frac{\hbar}{i}\left( f + x \frac{\partial f}{\partial x} \right) \\
&= - \frac{\hbar}{i} f
\end{align*}
holds for any function $f$.
By definition,
$[\hat{x}, \hat{p}_x] = - \frac{\hbar}{i}$.
$\Box$ \\

\emph{Proof of (b).}
\begin{align*}
[\hat{x}, \hat{p}_x^2]f
&= (\hat{x}\hat{p}_x^2 - \hat{p}_x^2 \hat{x})f \\
&= (\hat{x}\hat{p}_x^2)f - (\hat{p}_x^2 \hat{x})f \\
&= (\hat{x} \hat{p}_x)\left( \frac{\hbar}{i}\frac{\partial f}{\partial x} \right)
  - (\hat{p}_x^2)(xf) \\
&= (\hat{x})\left( \frac{\hbar}{i}\frac{\hbar}{i} \frac{\partial^2 f}{\partial x^2} \right)
  - (\hat{p}_x) \frac{\hbar}{i} \left( f + x \frac{\partial f}{\partial x} \right) \\
&= x \left( \frac{\hbar}{i}\frac{\hbar}{i} \frac{\partial^2 f}{\partial x^2} \right)
  - \frac{\hbar}{i} \frac{\hbar}{i} \left(
    \frac{\partial f}{\partial x} + \frac{\partial f}{\partial x}
  + x \frac{\partial^2 f}{\partial x^2} \right) \\
&= - \frac{\hbar}{i} \frac{\hbar}{i} \cdot 2 \frac{\partial f}{\partial x} \\
&= \left( 2 \hbar \frac{\partial}{\partial x} \right) f
\end{align*}
holds for any function $f$.
By definition,
$[\hat{x}, \hat{p}_x^2] = 2 \hbar \frac{\partial}{\partial x}$.
$\Box$ \\

\emph{Proof of (c).}
\begin{align*}
[\hat{x}, \hat{p}_y]f
&= (\hat{x}\hat{p}_y - \hat{p}_y \hat{x})f \\
&= (\hat{x}\hat{p}_y)f - (\hat{p}_y \hat{x})f \\
&= (\hat{x})\left( \frac{\hbar}{i}\frac{\partial f}{\partial y} \right)
  - (\hat{p}_y)(xf) \\
&= x \frac{\hbar}{i}\frac{\partial f}{\partial x}
  - \frac{\hbar}{i} \cdot x \frac{\partial f}{\partial y} \\
&= 0
\end{align*}
holds for any function $f$.
By definition,
$[\hat{x}, \hat{p}_y] = 0$.
$\Box$ \\

\emph{Proof of (d).}
\begin{align*}
[\hat{x}, \hat{V}(x,y,z)]f
&= (\hat{x}\hat{V}(x,y,z) - \hat{V}(x,y,z) \hat{x})f \\
&= (\hat{x}\hat{V}(x,y,z))f - (\hat{V}(x,y,z) \hat{x})f \\
&= \hat{x}(V(x,y,z)f) - \hat{V}(x,y,z)(xf) \\
&= x V(x,y,z)f - V(x,y,z) xf \\
&= 0
\end{align*}
holds for any function $f$.
By definition,
$[\hat{x}, \hat{V}(x,y,z)] = 0$.
$\Box$ \\





%%%%%%%%%%%%%%%%%%%%%%%%%%%%%%%%%%%%%%%%%%%%%%%%%%%%%%%%%%%%%%%%%%%%%%%%%%%%%%%%



\end{document}